revm: more progress on links for contract instructions

CoqOfRust/alloy_primitives/bits/links/fixed.v
@@ -5,6 +5,7 @@ Require Export alloy_primitives.bits.links.fixed_FixedBytes.
 Require Import alloy_primitives.bits.fixed.
 Require Import core.convert.links.mod.
 Require Import core.links.array.
+Require Import core.links.borrow.
 
 Module Impl_FixedBytes.
   Definition Self (N: Usize.t) : Set :=
@@ -62,3 +63,13 @@ Module Impl_From_U256_for_FixedBytes_32.
   Admitted.
 End Impl_From_U256_for_FixedBytes_32.
 Export Impl_From_U256_for_FixedBytes_32.
+
+(* impl<const N: usize> Borrow<[u8; N]> for FixedBytes<N> *)
+Module Impl_Borrow_Array_u8_N_for_FixedBytes_N.
+  Definition Self (N: Usize.t) : Set :=
+    FixedBytes.t N.
+
+  Instance run (N: Usize.t) : Borrow.Run (Self N) (array.t U8.t N).
+  Admitted.
+End Impl_Borrow_Array_u8_N_for_FixedBytes_N.
+Export Impl_Borrow_Array_u8_N_for_FixedBytes_N.
