CoqOfRust/core/ops/links/range.v
@@ -1,6 +1,7 @@
 Require Import CoqOfRust.CoqOfRust.
+Require Import CoqOfRust.links.M.
 Require Import core.links.cmp.
-Require Import links.M.
+Require Import core.ops.range.
 
 (*
   pub struct Range<Idx> {
@@ -36,6 +37,19 @@ Module Range.
   Defined.
   Smpl Add eapply of_ty : of_ty.
 End Range.
+
+Module Impl_Range.
+  Definition Self (Idx : Set) : Set :=
+    Range.t Idx.
+
+  (* pub fn is_empty(&self) -> bool *)
+  Instance run_is_empty {Idx : Set} `{Link Idx} (self : Ref.t Pointer.Kind.Ref (Self Idx)) :
+    Run.Trait
+      (ops.range.Impl_core_ops_range_Range_Idx.is_empty (Φ Idx)) [] [] [ φ self ]
+      bool.
+  Admitted.
+End Impl_Range.
+Export Impl_Range.
 
 (*
   pub enum Bound<T> {
