CoqOfRust/alloc/links/slice.v
@@ -1,0 +1,16 @@
+Require Import CoqOfRust.CoqOfRust.
+Require Import CoqOfRust.links.M.
+Require Import alloc.links.alloc.
+Require Import alloc.slice.
+Require Import alloc.vec.links.mod.
+
+Module Impl_Slice.
+  Definition Self (T : Set) : Set :=
+    list T.
+
+  (* pub fn to_vec(&self) -> Vec<T> *)
+  Instance run_to_vec (T : Set) `{Link T} (self : Ref.t Pointer.Kind.Ref (Self T)) :
+    Run.Trait (slice.Impl_slice_T.to_vec (Φ T)) [] [] [φ self] (Vec.t T Global.t).
+  Admitted.
+End Impl_Slice.
+Export Impl_Slice.
