CoqOfRust/core/ops/links/try_trait.v
@@ -1,0 +1,87 @@
+Require Import CoqOfRust.CoqOfRust.
+Require Import CoqOfRust.links.M.
+Require Import core.ops.links.control_flow.
+Require Import core.ops.try_trait.
+
+(*
+pub trait FromResidual<R = <Self as Try>::Residual> {
+    fn from_residual(residual: R) -> Self;
+}
+*)
+Module FromResidual.
+  Definition trait (Self : Set) `{Link Self} (R : Set) `{Link R} : TraitMethod.Header.t :=
+    ("core::ops::try_trait::FromResidual", [], [Φ R], Φ Self).
+
+  Definition Run_from_residual
+      (Self : Set) `{Link Self}
+      (R : Set) `{Link R} :
+      Set :=
+    TraitMethod.C (trait Self R) "from_residual" (fun method =>
+      forall (residual : R),
+      Run.Trait method [] [] [ φ residual ] Self
+    ).
+
+  Class Run (Self : Set) `{Link Self} (R : Set) `{Link R} : Set := {
+    from_residual : Run_from_residual Self R;
+  }.
+End FromResidual.
+
+(*
+pub trait Try: FromResidual {
+  type Output;
+  type Residual;
+
+  // Required methods
+  fn from_output(output: Self::Output) -> Self;
+  fn branch(self) -> ControlFlow<Self::Residual, Self::Output>;
+}
+*)
+Module Try.
+  Definition trait (Self : Set) `{Link Self} : TraitMethod.Header.t :=
+    ("core::ops::try_trait::Try", [], [], Φ Self).
+
+  Module Types.
+    Record t : Type := {
+      Output : Set;
+      Residual : Set;
+    }.
+
+    Class AreLinks (types : t) : Set := {
+      H_Output : Link types.(Output);
+      H_Residual : Link types.(Residual);
+    }.
+
+    Global Instance IsLinkOutput (types : t) (H : AreLinks types) : Link types.(Output) :=
+      H.(H_Output _).
+    Global Instance IsLinkResidual (types : t) (H : AreLinks types) : Link types.(Residual) :=
+      H.(H_Residual _).
+  End Types.
+
+  Definition Run_from_output
+      (Self : Set) `{Link Self}
+      (types : Types.t) `{Types.AreLinks types} :
+      Set :=
+    TraitMethod.C (trait Self) "from_output" (fun method =>
+      forall
+        (output : types.(Types.Output)),
+      Run.Trait method [] [] [ φ output ] Self
+    ).
+
+  Definition Run_branch
+      (Self : Set) `{Link Self}
+      (types : Types.t) `{Types.AreLinks types} :
+      Set :=
+    TraitMethod.C (trait Self) "branch" (fun method =>
+      forall
+        (self : Self),
+      Run.Trait method [] [] [ φ self ] (ControlFlow.t types.(Types.Residual) types.(Types.Output))
+    ).
+
+  Class Run (Self : Set) `{Link Self}
+      (types : Types.t) `{Types.AreLinks types} :
+      Set := {
+    run_FromResidual_for_Self : FromResidual.Run Self types.(Types.Residual);
+    from_output : Run_from_output Self types;
+    branch : Run_branch Self types;
+  }.
+End Try.
