CoqOfRust/revm/revm_interpreter/instructions/links/contract.v
@@ -1,21 +1,39 @@
 Require Import CoqOfRust.CoqOfRust.
 Require Import CoqOfRust.links.M.
 Require Import alloc.links.boxed.
+Require Import alloc.links.slice.
 Require Import alloy_primitives.bits.links.address.
 Require Import alloy_primitives.bits.links.fixed.
 Require Import alloy_primitives.bytes.links.mod.
+Require Import alloy_primitives.utils.links.mod.
 Require Import core.convert.links.mod.
+Require Import core.fmt.links.mod.
+Require Import core.links.borrow.
+Require Import core.links.cmp.
+Require Import core.links.option.
+Require Import core.links.panicking.
 Require Import core.links.result.
 Require Import core.num.links.mod.
+Require Import core.ops.links.control_flow.
 Require Import core.ops.links.range.
+Require Import core.slice.links.iter.
+Require Import revm.revm_bytecode.links.eof.
+Require Import revm.revm_context_interface.links.cfg.
 Require Import revm.revm_context_interface.links.host.
+Require Import revm.revm_interpreter.gas.links.calc.
+Require Import revm.revm_interpreter.gas.links.constants.
 Require Import revm.revm_interpreter.interpreter_action.links.call_inputs.
+Require Import revm.revm_interpreter.interpreter_action.links.eof_create_inputs.
+Require Import revm.revm_interpreter.interpreter.links.shared_memory.
 Require Import revm.revm_interpreter.links.gas.
 Require Import revm.revm_interpreter.links.interpreter.
 Require Import revm.revm_interpreter.links.interpreter_types.
 Require Import revm.revm_interpreter.instructions.contract.links.call_helpers.
 Require Import revm.revm_interpreter.instructions.contract.
+Require Import revm.revm_interpreter.instructions.links.utility.
 Require Import revm.revm_specification.links.hardfork.
+Require Import ruint.links.bytes.
+Require Import ruint.links.cmp.
 Require Import ruint.links.from.
 Require Import ruint.links.lib.
 
@@ -28,9 +46,7 @@ pub fn eofcreate<WIRE: InterpreterTypes, H: Host + ?Sized>(
 Instance run_eofcreate
   {WIRE H : Set} `{Link WIRE} `{Link H}
   {WIRE_types : InterpreterTypes.Types.t} `{InterpreterTypes.Types.AreLinks WIRE_types}
-  {H_types : Host.Types.t} `{Host.Types.AreLinks H_types}
   (run_InterpreterTypes_for_WIRE : InterpreterTypes.Run WIRE WIRE_types)
-  (run_Host_for_H : Host.Run H H_types)
   (interpreter : Ref.t Pointer.Kind.MutRef (Interpreter.t WIRE WIRE_types))
   (_host : Ref.t Pointer.Kind.MutRef H) :
   Run.Trait
@@ -38,6 +54,18 @@ Instance run_eofcreate
     unit.
 Proof.
   constructor.
+  destruct run_InterpreterTypes_for_WIRE eqn:?.
+  destruct run_StackTrait_for_Stack.
+  destruct run_LoopControl_for_Control.
+  destruct run_Immediates_for_Bytecode.
+  destruct run_Jumps_for_Bytecode.
+  destruct run_EofContainer_for_Bytecode.
+  destruct run_InputsTrait_for_Input.
+  destruct run_RuntimeFlag_for_RuntimeFlag.
+  destruct Impl_Clone_for_Bytes.run.
+  destruct Impl_Default_for_Bytes.run.
+  destruct Impl_Deref_for_Bytes.run.
+  destruct (Impl_Into_for_From_T.run Impl_From_Vec_u8_for_Bytes.run).
   run_symbolic.
 Admitted.
 
@@ -50,9 +78,7 @@ pub fn return_contract<H: Host + ?Sized>(
 Instance run_return_contract
   {WIRE H : Set} `{Link WIRE} `{Link H}
   {WIRE_types : InterpreterTypes.Types.t} `{InterpreterTypes.Types.AreLinks WIRE_types}
-  {H_types : Host.Types.t} `{Host.Types.AreLinks H_types}
   (run_InterpreterTypes_for_WIRE : InterpreterTypes.Run WIRE WIRE_types)
-  (run_Host_for_H : Host.Run H H_types)
   (interpreter : Ref.t Pointer.Kind.MutRef (Interpreter.t WIRE WIRE_types))
   (_host : Ref.t Pointer.Kind.MutRef H) :
   Run.Trait
@@ -60,6 +86,10 @@ Instance run_return_contract
     unit.
 Proof.
   constructor.
+  destruct run_InterpreterTypes_for_WIRE.
+  destruct run_StackTrait_for_Stack.
+  destruct run_Immediates_for_Bytecode.
+  destruct run_RuntimeFlag_for_RuntimeFlag.
   run_symbolic.
 Admitted.
 
@@ -69,12 +99,20 @@ pub fn extcall_input(interpreter: &mut Interpreter<impl InterpreterTypes>) -> Op
 Instance run_extcall_input
   {WIRE : Set} `{Link WIRE}
   {WIRE_types : InterpreterTypes.Types.t} `{InterpreterTypes.Types.AreLinks WIRE_types}
+  (run_InterpreterTypes_for_WIRE : InterpreterTypes.Run WIRE WIRE_types)
   (interpreter : Ref.t Pointer.Kind.MutRef (Interpreter.t WIRE WIRE_types)) :
   Run.Trait
     instructions.contract.extcall_input [] [ Φ WIRE ] [ φ interpreter ]
     (option Bytes.t).
 Proof.
   constructor.
+  destruct run_InterpreterTypes_for_WIRE eqn:?.
+  destruct run_StackTrait_for_Stack.
+  destruct run_MemoryTrait_for_Memory.
+  destruct (Impl_Try_for_Option.run Bytes.t).
+  destruct run_FromResidual_for_Self.
+  destruct (Impl_Try_for_Option.run (Range.t Usize.t)).
+  destruct (Impl_AsRef_for_Slice.run U8.t).
   run_symbolic.
 Admitted.
 
@@ -93,12 +131,20 @@ Instance run_extcall_gas_calc
   (run_InterpreterTypes_for_WIRE : InterpreterTypes.Run WIRE WIRE_types)
   (run_Host_for_H : Host.Run H H_types)
   (interpreter : Ref.t Pointer.Kind.MutRef (Interpreter.t WIRE WIRE_types))
-  (host : Ref.t Pointer.Kind.MutRef H) :
+  (host : Ref.t Pointer.Kind.MutRef H)
+  (target : Address.t)
+  (transfers_value : bool) :
   Run.Trait
-    instructions.contract.extcall_gas_calc [] [ Φ WIRE; Φ H ] [ φ interpreter; φ host ]
+    instructions.contract.extcall_gas_calc
+      [] [ Φ WIRE; Φ H ] [ φ interpreter; φ host; φ target; φ transfers_value ]
     (option U64.t).
 Proof.
   constructor.
+  destruct run_InterpreterTypes_for_WIRE.
+  destruct run_StackTrait_for_Stack.
+  destruct run_LoopControl_for_Control.
+  destruct run_RuntimeFlag_for_RuntimeFlag.
+  destruct run_Host_for_H.
   run_symbolic.
 Admitted.
 
@@ -110,12 +156,17 @@ pub fn pop_extcall_target_address(
 Instance run_pop_extcall_target_address
   {WIRE : Set} `{Link WIRE}
   {WIRE_types : InterpreterTypes.Types.t} `{InterpreterTypes.Types.AreLinks WIRE_types}
+  (run_InterpreterTypes_for_WIRE : InterpreterTypes.Run WIRE WIRE_types)
   (interpreter : Ref.t Pointer.Kind.MutRef (Interpreter.t WIRE WIRE_types)) :
   Run.Trait
     instructions.contract.pop_extcall_target_address [] [ Φ WIRE ] [ φ interpreter ]
     (option Address.t).
 Proof.
   constructor.
+  destruct run_InterpreterTypes_for_WIRE.
+  destruct run_StackTrait_for_Stack.
+  destruct Impl_From_U256_for_FixedBytes_32.run.
+  destruct (Impl_Iterator_for_Iter.run U8.t).
   run_symbolic.
 Admitted.
 
@@ -138,9 +189,13 @@ Instance run_extcall
     unit.
 Proof.
   constructor.
+  destruct run_InterpreterTypes_for_WIRE eqn:?.
+  destruct run_StackTrait_for_Stack.
+  destruct run_LoopControl_for_Control.
+  destruct run_InputsTrait_for_Input.
+  destruct run_RuntimeFlag_for_RuntimeFlag.
   run_symbolic.
 Admitted.
-
 
 (*
 pub fn extdelegatecall<WIRE: InterpreterTypes, H: Host + ?Sized>(
@@ -161,6 +216,10 @@ Instance run_extdelegatecall
     unit.
 Proof.
   constructor.
+  destruct run_InterpreterTypes_for_WIRE eqn:?.
+  destruct run_LoopControl_for_Control.
+  destruct run_InputsTrait_for_Input.
+  destruct run_RuntimeFlag_for_RuntimeFlag.
   run_symbolic.
 Admitted.
 
@@ -183,9 +242,12 @@ Instance run_extstaticcall
     unit.
 Proof.
   constructor.
+  destruct run_InterpreterTypes_for_WIRE eqn:?.
+  destruct run_LoopControl_for_Control.
+  destruct run_InputsTrait_for_Input.
+  destruct run_RuntimeFlag_for_RuntimeFlag.
   run_symbolic.
 Admitted.
-
 
 (*
 pub fn create<WIRE: InterpreterTypes, const IS_CREATE2: bool, H: Host + ?Sized>(
@@ -194,6 +256,7 @@ pub fn create<WIRE: InterpreterTypes, const IS_CREATE2: bool, H: Host + ?Sized>(
 )
 *)
 Instance run_create
+  (IS_CREATE2 : bool)
   {WIRE H : Set} `{Link WIRE} `{Link H}
   {WIRE_types : InterpreterTypes.Types.t} `{InterpreterTypes.Types.AreLinks WIRE_types}
   {H_types : Host.Types.t} `{Host.Types.AreLinks H_types}
@@ -202,13 +265,22 @@ Instance run_create
   (interpreter : Ref.t Pointer.Kind.MutRef (Interpreter.t WIRE WIRE_types))
   (host : Ref.t Pointer.Kind.MutRef H) :
   Run.Trait
-    instructions.contract.create [] [ Φ WIRE; Φ H ] [ φ interpreter; φ host ]
+    instructions.contract.create [ φ IS_CREATE2 ] [ Φ WIRE; Φ H ] [ φ interpreter; φ host ]
     unit.
 Proof.
   constructor.
+  destruct run_InterpreterTypes_for_WIRE.
+  destruct run_StackTrait_for_Stack.
+  destruct run_MemoryTrait_for_Memory.
+  destruct run_LoopControl_for_Control.
+  destruct run_InputsTrait_for_Input.
+  destruct run_RuntimeFlag_for_RuntimeFlag.
+  destruct run_Host_for_H.
+  destruct run_CfgGetter_for_Self.
+  destruct run_Cfg_for_Cfg.
+  destruct (Impl_AsRef_for_Slice.run U8.t).
   run_symbolic.
 Admitted.
-
 
 (*
 pub fn call<WIRE: InterpreterTypes, H: Host + ?Sized>(
@@ -229,9 +301,16 @@ Instance run_call
     unit.
 Proof.
   constructor.
+  destruct run_InterpreterTypes_for_WIRE eqn:?.
+  destruct run_StackTrait_for_Stack.
+  destruct run_LoopControl_for_Control.
+  destruct run_InputsTrait_for_Input.
+  destruct run_RuntimeFlag_for_RuntimeFlag.
+  destruct run_Host_for_H.
+  destruct (TryFrom_Uint_for_u64.run {| Integer.value := 256 |} {| Integer.value := 4 |}).
+  destruct Impl_IntoAddress_for_U256.run.
   run_symbolic.
 Admitted.
-
 
 (*
 pub fn call_code<WIRE: InterpreterTypes, H: Host + ?Sized>(
@@ -252,6 +331,15 @@ Instance run_call_code
     unit.
 Proof.
   constructor.
+  destruct run_InterpreterTypes_for_WIRE eqn:?.
+  destruct run_StackTrait_for_Stack.
+  destruct run_MemoryTrait_for_Memory.
+  destruct run_LoopControl_for_Control.
+  destruct run_InputsTrait_for_Input.
+  destruct run_RuntimeFlag_for_RuntimeFlag.
+  destruct run_Host_for_H.
+  destruct Impl_From_U256_for_FixedBytes_32.run.
+  destruct (TryFrom_Uint_for_u64.run {| Integer.value := 256 |} {| Integer.value := 4 |}).
   run_symbolic.
 Admitted.
 
@@ -275,6 +363,14 @@ Instance run_delegate_call
     unit.
 Proof.
   constructor.
+  destruct run_InterpreterTypes_for_WIRE eqn:?.
+  destruct run_StackTrait_for_Stack.
+  destruct run_LoopControl_for_Control.
+  destruct run_InputsTrait_for_Input.
+  destruct run_RuntimeFlag_for_RuntimeFlag.
+  destruct run_Host_for_H.
+  destruct Impl_From_U256_for_FixedBytes_32.run.
+  destruct (TryFrom_Uint_for_u64.run {| Integer.value := 256 |} {| Integer.value := 4 |}).
   run_symbolic.
 Admitted.
 
